src/goose_lang/dist_adequacy.v
@@ -7,13 +7,13 @@ From Perennial.goose_lang Require Import adequacy lang.
 From Perennial.goose_lang Require Import crash_modality.
 Set Default Proof Using "Type".
 
-Theorem goose_dist_adequacy `{ffi_sem: ffi_semantics} `{!ffi_interp ffi} {Hffi_adequacy:ffi_interp_adequacy}
-        Σ `{hPre: !gooseGpreS Σ} (ebσs : list node_init_cfg)
-        g φinv (HINITG: ffi_initgP g.(global_world)) (HINIT: ∀ σ, σ ∈ init_local_state <$> ebσs → ffi_initP σ.(world) g.(global_world))
-        {go_gctx : GoGlobalContext} :
-  (∀ `(HG : !gooseGlobalGS Σ),
-      ⊢
-        ffi_global_start goose_ffiGlobalGS g.(global_world) ={⊤}=∗
+Theorem goose_dist_adequacy `{ffi_sem: ffi_semantics}
+  `{!ffi_interp ffi} {Hffi_adequacy:ffi_interp_adequacy}
+  {go_gctx : GoGlobalContext}
+  Σ `{hPre: !gooseGpreS Σ} (ebσs : list node_init_cfg)
+  g φinv (HINITG: ffi_initgP g.(global_world)) (HINIT: ∀ σ, σ ∈ init_local_state <$> ebσs → ffi_initP σ.(world) g.(global_world))
+  : (∀ `(HG : !gooseGlobalGS Σ),
+      ⊢ ffi_global_start goose_ffiGlobalGS g.(global_world) ={⊤}=∗
         wpd ⊤ ebσs ∗
         (∀ g, ffi_global_ctx goose_ffiGlobalGS g.(global_world) -∗ |={⊤, ∅}=> ⌜ φinv g ⌝)) →
   dist_adequate (CS := goose_crash_lang) ebσs g (λ g, φinv g).
@@ -25,7 +25,7 @@ Proof.
   iMod (credit_name_init (crash_borrow_ginv_number)) as (name_credit) "(Hcred_auth&Hcred&Htok)".
   iMod (proph_map_init κs g.(used_proph_id)) as (proph_names) "Hproph".
 
-  set (hG := GooseGlobalGS _ _ _ proph_names (creditGS_update_pre _ _ name_credit) ffi_namesg).
+  set (hG := GooseGlobalGS _ _ proph_names (creditGS_update_pre _ _ name_credit) ffi_namesg).
 
   iExists global_state_interp, fork_post.
   iExists _, _.
@@ -36,7 +36,6 @@ Proof.
   { rewrite /crash_borrow_ginv. iApply (inv_alloc _). iNext. eauto. }
   iModIntro.
   iFrame "Hgw Hinv Hcred_auth Htok Hproph".
-  FIXME:
   iSplitR; first by eauto.
   iSplitL "Hwp"; last first.
   { iIntros (???) "Hσ".
@@ -51,13 +50,12 @@ Proof.
   iMod (ffi_local_init _ _ σ.(init_local_state).(world)) as (ffi_names) "(Hw&Hstart)".
   { eapply HINIT. apply list_elem_of_fmap. eexists. split; first done.
     eapply list_elem_of_lookup_2. done. }
-  iMod (trace_name_init σ.(init_local_state).(trace) σ.(init_local_state).(oracle)) as (name_trace) "(Htr&Htrfrag&Hor&Hofrag)".
-  iMod (globals_name_init _ σ.(init_local_state).(globals)) as (globals_name) "(Hg & Hg_auth)".
-  set (hL := GooseLocalGS Σ Hc ffi_names (na_heapGS_update_pre _ name_na_heap) (traceGS_update_pre Σ _ name_trace)
-                          (globalsGS_update_pre Σ _ globals_name)
+  iMod (go_state_init) as (globals_name) "(Hg & Hg_auth)".
+  set (hL := GooseLocalGS Σ Hc ffi_names σ.(init_local_state).(go_state).(go_lctx) (na_heapGS_update_pre _ name_na_heap)
+                          (go_stateGS_update_pre Σ _ globals_name)
       ).
 
-  iMod ("H" $! hL with "[$] [$] [$] [$]") as (Φ Φrx Φinv) "Hwpr".
+  iMod ("H" $! hL with "[$] [$]") as (Φ Φrx Φinv) "Hwpr".
   iModIntro. iExists state_interp, _, _, _.
   iSplitR "Hwpr"; first by iFrame.
   rewrite /wpr//=.
@@ -66,6 +64,7 @@ Qed.
 Section failstop.
 
 Context `{ffi_sem: ffi_semantics} `{!ffi_interp ffi} {Hffi_adequacy:ffi_interp_adequacy}.
+Context {go_gctx : GoGlobalContext}.
 
 (* We can model failstop execution by just having the restart thread be a trivial program that just halts.
    Thus, a node "restarts" after a crash but it does not do anything. *)
@@ -88,9 +87,7 @@ Theorem goose_dist_adequacy_failstop
            let σ := snd ebσ in
            ∀ `(hL: !gooseLocalGS Σ),
              ffi_local_start (goose_ffiLocalGS) σ.(world) -∗
-             own_globals (DfracOwn 1) σ.(globals) -∗
-             trace_frag σ.(trace) -∗
-             oracle_frag σ.(oracle) ={⊤}=∗
+             own_go_state σ.(go_state).(package_state) ={⊤}=∗
              ∃ Φ, wp NotStuck ⊤ e Φ) ∗
         (∀ g, ffi_global_ctx goose_ffiGlobalGS g.(global_world) -∗ |={⊤, ∅}=> ⌜ φinv g ⌝)) →
   dist_adequate_failstop ebσs g (λ g, φinv g).
@@ -105,7 +102,7 @@ Proof.
   iApply big_sepL_fmap. simpl.
   iApply (big_sepL_mono with "Hwp").
   iIntros (i (e&σ) Hlookup) "H".
-  iIntros (HL) "Hffi Hglobals Htrace Horacle". iMod ("H" $! HL with "[$] [$] [$] [$]") as "Hwp".
+  iIntros (HL) "Hffi Hglobals". iMod ("H" $! HL with "[$] [$]") as "Hwp".
   iDestruct "Hwp" as (Φ) "H". simpl.
   iModIntro. iExists Φ, (λ _ _, True%I), (λ _, True%I).
   set (Hheao := HeapGS _ HG HL).
