src/goose_lang/dist_lifting.v
@@ -10,13 +10,12 @@ Section wpd_definitions.
 Context `{ffi_sem: ffi_semantics}.
 Context `{interp: !ffi_interp ffi}.
 Context `{@ffi_interp_adequacy ffi interp ext ffi_sem}.
+Context {go_gctx : GoGlobalContext}.
 
 Definition wpd `{hG: !gooseGlobalGS Σ} (E: coPset) (ers: list node_init_cfg) :=
   ([∗ list] i↦σ ∈ ers, ∀ `(hG: !gooseLocalGS Σ),
     ffi_local_start (goose_ffiLocalGS) σ.(init_local_state).(world) -∗
-    own_go_state σ.(init_local_state).(go_state).(package_state) -∗
-    trace_frag σ.(init_local_state).(trace) -∗
-    oracle_frag σ.(init_local_state).(oracle) ={E}=∗
+    own_go_state σ.(init_local_state).(go_state).(package_state) ={E}=∗
     ∃ Φ Φrx Φinv, wpr NotStuck E σ.(init_thread) σ.(init_restart) Φ Φinv Φrx)%I.
 
 Lemma wpd_compose `{hG: !gooseGlobalGS Σ} E ers1 ers2 :
